Remove old parsing algorithm

RegexPosix/POSIX.lean
@@ -1,73 +1,37 @@
 import RegexPosix.Value
 
+open Parse
 open Regex
-open Value
 
 universe u
 
 variable {α : Type u}
 
-inductive POSIX : Regex α → Value α → Prop
-  | epsilon : POSIX epsilon empty
-  | char (c : α) : POSIX (char c) (char c)
-  | left {r₁ r₂ : Regex α} {v : Value α} :
-    POSIX r₁ v →
-    POSIX (plus r₁ r₂) (left v)
-  | right {r₁ r₂ : Regex α} {v : Value α} :
-    POSIX r₂ v →
-    ¬r₁.Matches v.flat →
-    POSIX (plus r₁ r₂) (right v)
-  | mul {r₁ r₂ : Regex α} {v₁ v₂ : Value α} :
-    POSIX r₁ v₁ →
-    POSIX r₂ v₂ →
-    ¬(∃ s₃ s₄, s₃ ≠ [] ∧ s₃ ++ s₄ = v₂.flat ∧ r₁.Matches (v₁.flat ++ s₃) ∧ r₂.Matches s₄) →
-    POSIX (mul r₁ r₂) (seq v₁ v₂)
-  | star_nil {r : Regex α} :
-    POSIX (star r) (stars [])
-  | stars {r : Regex α} {v : Value α} {vs : List (Value α)} :
-    POSIX r v →
-    POSIX (star r) (stars vs) →
-    v.flat ≠ [] →
-    ¬(∃ s₃ s₄, s₃ ≠ [] ∧ s₃ ++ s₄ = (stars vs).flat ∧ r.Matches (v.flat ++ s₃) ∧ (star r).Matches s₄) →
-    POSIX (star r) (stars (v::vs))
-
-inductive POSIX' : {r : Regex α} → Parse r → Prop
-  | epsilon : POSIX' Parse.empty
-  | char (c : α) : POSIX' (Parse.char c)
+inductive POSIX : {r : Regex α} → Parse r → Prop
+  | epsilon : POSIX empty
+  | char (c : α) : POSIX (char c)
   | left {r₁ : Regex α} {p : Parse r₁} :
-    POSIX' p →
-    POSIX' p.left
+    POSIX p →
+    POSIX p.left
   | right {r₁ r₂ : Regex α} {p : Parse r₂} :
-    POSIX' p →
+    POSIX p →
     ¬r₁.Matches p.flat →
-    @POSIX' (r₁.plus r₂) p.right
+    @POSIX (r₁.plus r₂) p.right
   | mul {r₁ r₂ : Regex α} {p₁ : Parse r₁} {p₂ : Parse r₂} :
-    POSIX' p₁ →
-    POSIX' p₂ →
+    POSIX p₁ →
+    POSIX p₂ →
     ¬(∃ s₃ s₄, s₃ ≠ [] ∧ s₃ ++ s₄ = p₂.flat ∧ r₁.Matches (p₁.flat ++ s₃) ∧ r₂.Matches s₄) →
-    POSIX' (p₁.seq p₂)
+    POSIX (p₁.seq p₂)
   | star_nil :
-    POSIX' Parse.star_nil
+    POSIX star_nil
   | stars {r : Regex α} {p : Parse r} {ps : Parse (star r)} :
-    POSIX' p →
-    POSIX' ps →
+    POSIX p →
+    POSIX ps →
     p.flat ≠ [] →
     ¬(∃ s₃ s₄, s₃ ≠ [] ∧ s₃ ++ s₄ = ps.flat ∧ r.Matches (p.flat ++ s₃) ∧ (star r).Matches s₄) →
-    POSIX' (p.star_cons ps)
+    POSIX (p.star_cons ps)
 
-theorem POSIX.inhab {r : Regex α} {v : Value α} : POSIX r v → Inhab v r
-  | epsilon => Inhab.empty
-  | char c => Inhab.char c
-  | left h => Inhab.left (inhab h)
-  | right h hn => Inhab.right (inhab h)
-  | mul h₁ h₂ hn => Inhab.seq (inhab h₁) (inhab h₂)
-  | star_nil => Inhab.star_nil
-  | stars h₁ h₂ hv hn => Inhab.stars (inhab h₁) (inhab h₂)
-
-theorem POSIX.matches {r : Regex α} {v : Value α} : POSIX r v → r.Matches v.flat :=
-  fun h => h.inhab.matches
-
-theorem POSIX'.matches {r : Regex α} {p : Parse r} : POSIX' p → r.Matches p.flat :=
+theorem POSIX.matches {r : Regex α} {p : Parse r} : POSIX p → r.Matches p.flat :=
   fun _ => p.matches
 
 theorem longest_split_unique {r₁ r₂ : Regex α} {s₁₁ s₁₂ s₂₁ s₂₂ : List α}
@@ -94,7 +58,7 @@ theorem longest_split_unique {r₁ r₂ : Regex α} {s₁₁ s₁₂ s₂₁ s�
     | cons x xs =>
       exact absurd hr₁₂ (h₂ (x::xs) (by simp) s₁₂ rfl hr₁₁)
 
-theorem POSIX'.unique {r : Regex α} {p₁ p₂ : Parse r} (hp : p₁.flat = p₂.flat) (h₁ : POSIX' p₁) (h₂ : POSIX' p₂) :
+theorem POSIX.unique {r : Regex α} {p₁ p₂ : Parse r} (hp : p₁.flat = p₂.flat) (h₁ : POSIX p₁) (h₂ : POSIX p₂) :
   p₁ = p₂ := by
   induction h₁ with
   | epsilon =>
@@ -106,7 +70,7 @@ theorem POSIX'.unique {r : Regex α} {p₁ p₂ : Parse r} (hp : p₁.flat = p�
   | left h₁ ih =>
     cases h₂ with
     | left h₂ =>
-      rw [Parse.left.injEq]
+      rw [left.injEq]
       simp at hp
       exact ih hp h₂
     | right h₂ hn =>
@@ -120,7 +84,7 @@ theorem POSIX'.unique {r : Regex α} {p₁ p₂ : Parse r} (hp : p₁.flat = p�
       rw [hp] at hn
       exact absurd h₂.matches hn
     | right h₂ hn' =>
-      rw [Parse.right.injEq]
+      rw [right.injEq]
       simp at hp
       exact ih hp h₂
   | mul h₁₁ h₁₂ hs₁ ih₁ ih₂ =>
@@ -143,59 +107,6 @@ theorem POSIX'.unique {r : Regex α} {p₁ p₂ : Parse r} (hp : p₁.flat = p�
     | stars h₂₁ h₂₂ hp₂ hs₂ =>
       simp at hp
       have hv' := longest_split_unique hp h₁₁.matches h₁₂.matches h₂₁.matches h₂₂.matches hs₁ hs₂
-      have ih₂ := ih₂ hv'.right h₂₂
-      simp at ih₂
-      rw [ih₁ hv'.left h₂₁, ih₂]
-
-theorem POSIX.unique {r : Regex α} {v₁ v₂ : Value α} (hv : v₁.flat = v₂.flat) (h₁ : POSIX r v₁) (h₂ : POSIX r v₂) :
-  v₁ = v₂ := by
-  induction h₁ generalizing v₂ with
-  | epsilon =>
-    cases h₂
-    rfl
-  | char c =>
-    cases h₂
-    rfl
-  | left h₁ ih =>
-    cases h₂ with
-    | left h₂ =>
-      rw [left.injEq]
-      simp at hv
-      exact ih hv h₂
-    | right h₂ hn =>
-      simp at hv
-      rw [←hv] at hn
-      exact absurd (POSIX.matches h₁) hn
-  | right h₁ hn ih =>
-    cases h₂ with
-    | left h₂ =>
-      simp at hv
-      rw [hv] at hn
-      exact absurd (POSIX.matches h₂) hn
-    | right h₂ hn' =>
-      rw [right.injEq]
-      simp at hv
-      exact ih hv h₂
-  | mul h₁₁ h₁₂ hn₁ ih₁ ih₂ =>
-    cases h₂ with
-    | mul h₂₁ h₂₂ hn₂ =>
-      simp at hv
-      have hv' := longest_split_unique hv (POSIX.matches h₁₁) (POSIX.matches h₁₂) (POSIX.matches h₂₁) (POSIX.matches h₂₂) hn₁ hn₂
-      rw [ih₁ hv'.left h₂₁, ih₂ hv'.right h₂₂]
-  | star_nil =>
-    cases h₂ with
-    | star_nil => rfl
-    | stars _ _ hv' =>
-      simp at hv
-      exact absurd hv.left hv'
-  | stars h₁₁ h₁₂ hv' hn₁ ih₁ ih₂ =>
-    cases h₂ with
-    | star_nil =>
-      simp at hv
-      exact absurd hv.left hv'
-    | stars h₂₁ h₂₂ _ hn₂ =>
-      simp at hv
-      have hv' := longest_split_unique hv (POSIX.matches h₁₁) (POSIX.matches h₁₂) (POSIX.matches h₂₁) (POSIX.matches h₂₂) hn₁ hn₂
       have ih₂ := ih₂ hv'.right h₂₂
       simp at ih₂
       rw [ih₁ hv'.left h₂₁, ih₂]
