RegexPosix/Parse.lean
@@ -1,66 +1,29 @@
 import RegexPosix.Value
 import Mathlib.Tactic.GeneralizeProofs
 
-open Value
+open Parse
 open Regex
 
 universe u
 
 variable {α : Type u}
 
-def Regex.mkeps : (r : Regex α) → r.nullable → (Σ' v : Value α, Inhab v r)
-  | epsilon, _ => ⟨Value.empty, Inhab.empty⟩
-  | plus r₁ r₂, hn =>
-    if hn₁ : r₁.nullable
-      then
-        have ⟨v₁, h₁⟩ := mkeps r₁ hn₁
-        ⟨Value.left v₁, Inhab.left h₁⟩
-      else
-        have hn₂ := (Bool.or_eq_true_iff.mp hn).resolve_left hn₁
-        have ⟨v₂, h₂⟩ := mkeps r₂ hn₂
-        ⟨Value.right v₂, Inhab.right h₂⟩
-  | mul r₁ r₂, hn =>
-    have ⟨v₁, h₁⟩ := mkeps r₁ (Bool.and_elim_left hn)
-    have ⟨v₂, h₂⟩ := mkeps r₂ (Bool.and_elim_right hn)
-    ⟨Value.seq v₁ v₂, Inhab.seq h₁ h₂⟩
-  | star _, _ => ⟨Value.stars [], Inhab.star_nil⟩
-
-theorem mkeps_flat {α : Type u} {r : Regex α} (hn : r.nullable) :
-  (r.mkeps hn).fst.flat = [] := by
-  induction r with
-  | emptyset => simp at hn
-  | epsilon =>
-    simp only [mkeps, Value.flat]
-  | char c => simp at hn
-  | plus r₁ r₂ ih₁ ih₂ =>
-    simp at hn
-    simp [mkeps]
-    split_ifs with hn'
-    · rw [Value.flat, ih₁]
-    · rw [Value.flat, ih₂]
-  | mul r₁ r₂ ih₁ ih₂ =>
-    simp at hn
-    simp [mkeps]
-    rw [ih₁, ih₂, and_self]
-  | star r ih => simp [mkeps]
-
-def mkeps' : {r : Regex α} → r.nullable → Parse r
-  | epsilon, _ => Parse.empty
+def mkeps : {r : Regex α} → r.nullable → Parse r
+  | epsilon, _ => empty
   | plus r₁ _, hn =>
     if hn₁ : r₁.nullable
-      then
-        Parse.left (mkeps' hn₁)
+      then left (mkeps hn₁)
       else
         have hn₂ := (Bool.or_eq_true_iff.mp hn).resolve_left hn₁
-        Parse.right (mkeps' hn₂)
+        right (mkeps hn₂)
   | mul _ _, hn =>
     have ⟨hn₁, hn₂⟩ := Bool.and_eq_true_iff.mp hn
-    Parse.seq (mkeps' hn₁) (mkeps' hn₂)
-  | star _, _ => Parse.star_nil
+    seq (mkeps hn₁) (mkeps hn₂)
+  | star _, _ => star_nil
 
-theorem mkeps'_flat {r : Regex α} {hn : r.nullable} :
-  (mkeps' hn).flat = [] := by
-  fun_induction mkeps' with
+theorem mkeps_flat {r : Regex α} {hn : r.nullable} :
+  (mkeps hn).flat = [] := by
+  fun_induction mkeps with
   | case1 => rfl
   | case2 r₁ r₂ hn hn₁ ih₁ =>
     simp only [Parse.flat, ih₁]
@@ -72,68 +35,37 @@ theorem mkeps'_flat {r : Regex α} {hn : r.nullable} :
 
 variable [DecidableEq α]
 
-def inj' : {r : Regex α} → (c : α) → Parse (r.deriv c) → Parse r
-  | .char d, _c, _ => Parse.char d
-  | .plus r₁ r₂, c, Parse.left p => Parse.left (inj' c p)
-  | .plus r₁ r₂, c, Parse.right p => Parse.right (inj' c p)
+def inj : {r : Regex α} → (c : α) → Parse (r.deriv c) → Parse r
+  | .char d, _c, _ => char d
+  | .plus r₁ r₂, c, left p => left (inj c p)
+  | .plus r₁ r₂, c, right p => right (inj c p)
   | .mul r₁ _, c, p =>
     if hn₁ : r₁.nullable
       then
-        match (deriv_mul_nullable hn₁) ▸ p with
-        | Parse.left (Parse.seq p₁ p₂) =>
-          Parse.seq (inj' c p₁) p₂
-        | Parse.right p₂ =>
-          Parse.seq (mkeps' hn₁) (inj' c p₂)
+        match p.cast (deriv_mul_nullable hn₁) with
+        | left (seq p₁ p₂) => seq (inj c p₁) p₂
+        | right p₂ => seq (mkeps hn₁) (inj c p₂)
       else
-        match (deriv_mul_not_nullable hn₁) ▸ p with
-        | Parse.seq p₁ p₂ =>
-          Parse.seq (inj' c p₁) p₂
-  | .star r, c, Parse.seq p ps =>
-    Parse.star_cons (inj' c p) ps
+        match p.cast (deriv_mul_not_nullable hn₁) with
+        | seq p₁ p₂ => seq (inj c p₁) p₂
+  | .star r, c, seq p ps => star_cons (inj c p) ps
 
-def inj : (r : Regex α) → (c : α) → (Σ' v : Value α, Inhab v (r.deriv c)) → (Σ' v : Value α, Inhab v r)
-  | .char d, c, ⟨v, h⟩ => ⟨Value.char d, Inhab.char d⟩
-  | .plus r₁ r₂, c, ⟨Value.left v₁, h₁⟩ =>
-    have ⟨v₁, h₁⟩ := inj r₁ c ⟨v₁, inhab_left h₁⟩
-    ⟨v₁.left, h₁.left⟩
-  | .plus r₁ r₂, c, ⟨Value.right v₂, h₂⟩ =>
-    have ⟨v₂, h₂⟩ := inj r₂ c ⟨v₂, inhab_right h₂⟩
-    ⟨v₂.right, h₂.right⟩
-  | .mul r₁ r₂, c, ⟨v, h⟩ => by
-    rw [Regex.deriv] at h
-    split_ifs at h with hn
-    · match v with
-      | Value.left (Value.seq v₁ v₂) =>
-        have ⟨v₁, h₁⟩ := inj r₁ c ⟨v₁, inhab_seq_fst (inhab_left h)⟩
-        exact ⟨v₁.seq v₂, h₁.seq (inhab_seq_snd (inhab_left h))⟩
-      | Value.right v₂ =>
-        have ⟨v₂, h₂⟩ := inj r₂ c ⟨v₂, inhab_right h⟩
-        have ⟨v₁, h₁⟩ := r₁.mkeps hn
-        exact ⟨v₁.seq v₂, h₁.seq h₂⟩
-    · match v with
-      | Value.seq v₁ v₂ =>
-        have ⟨v₁, h₁⟩ := inj r₁ c ⟨v₁, inhab_seq_fst h⟩
-        exact ⟨v₁.seq v₂, h₁.seq (inhab_seq_snd h)⟩
-  | .star r, c, ⟨Value.seq v (Value.stars vs), h⟩ =>
-    have ⟨v, hv⟩ := inj r c ⟨v, inhab_seq_fst h⟩
-    ⟨Value.stars (v :: vs), Inhab.stars hv (inhab_seq_snd h)⟩
-
-theorem inj'_flat {r : Regex α} {c : α} {p : Parse (r.deriv c)} :
-  (inj' c p).flat = c::p.flat := by
-  fun_induction inj' with
+theorem inj_flat {r : Regex α} {c : α} {p : Parse (r.deriv c)} :
+  (inj c p).flat = c::p.flat := by
+  fun_induction inj with
   | case1 d c p =>
     generalize hr : (Regex.char d).deriv c = r' at p
     rw [Regex.deriv] at hr
     split_ifs at hr with hc
     · subst hr hc
       cases p
-      simp only [Parse.flat]
+      simp only [flat]
     · subst hr
       nomatch p
   | case2 r₁ r₂ c p ih =>
-    simp only [Parse.flat, ih]
+    simp only [flat, ih]
   | case3 r₁ r₂ c p ih =>
-    simp only [Parse.flat, ih]
+    simp only [flat, ih]
   | case4 r₁ r₂ c hn p₁ p₂ p heq ih₁ =>
     generalize_proofs k at heq
     generalize hr : (r₁.mul r₂).deriv c = r' at *
@@ -145,7 +77,7 @@ theorem inj'_flat {r : Regex α} {c : α} {p : Parse (r.deriv c)} :
     generalize hr : (r₁.mul r₂).deriv c = r' at *
     simp [deriv, hn] at hr
     subst hr heq
-    simp [mkeps'_flat, ih₂]
+    simp [mkeps_flat, ih₂]
   | case6 r₁ r₂ c hn p₁ p₂ p heq ih₁ =>
     generalize_proofs k at heq
     generalize hr : (r₁.mul r₂).deriv c = r' at *
@@ -155,100 +87,29 @@ theorem inj'_flat {r : Regex α} {c : α} {p : Parse (r.deriv c)} :
   | case7 r c p ps ih =>
     simp [ih]
 
-theorem inj_flat {r : Regex α} {c : α} {v : Value α} (hv : Inhab v (r.deriv c)) :
-  (inj r c ⟨v, hv⟩).fst.flat = c::v.flat := by
-  induction r generalizing v with
-  | emptyset => nomatch hv
-  | epsilon => nomatch hv
-  | char d =>
-    rw [deriv] at hv
-    split_ifs at hv with hc
-    · cases hv
-      simp [inj, hc]
-    · nomatch hv
-  | plus r₁ r₂ ih₁ ih₂ =>
-    cases hv with
-    | left hv =>
-      simp [inj, ih₁]
-    | right hv =>
-      simp [inj, ih₂]
-  | mul r₁ r₂ ih₁ ih₂ =>
-    rw [deriv] at hv
-    split_ifs at hv with hn
-    · match v with
-      | Value.left (Value.seq v₁ v₂) =>
-        simp [inj, hn, ih₁]
-      | Value.right v₂ =>
-        simp [inj, hn, ih₂]
-        exact mkeps_flat _
-    · match v with
-      | Value.seq v₁ v₂ =>
-        simp [inj, hn, ih₁]
-  | star r ih =>
-    match v with
-    | Value.seq v (Value.stars vs) =>
-      simp [inj, ih]
-
-def injs' : {r : Regex α} → (s : List α) → (Parse (r.derivs s)) → Parse r
+def injs : {r : Regex α} → (s : List α) → (Parse (r.derivs s)) → Parse r
   | _, [], p => p
-  | _, c::s, p => inj' c (injs' s p)
+  | _, c::s, p => inj c (injs s p)
 
-def injs : (r : Regex α) → (s : List α) → (Σ' v : Value α, Inhab v (r.derivs s)) → (Σ' v' : Value α, Inhab v' r)
-  | _, [], h => h
-  | r, c::s, h => inj r c (injs (r.deriv c) s h)
-
-theorem injs'_flat {r : Regex α} {s : List α} {p : Parse (r.derivs s)} :
-  (injs' s p).flat = s ++ p.flat := by
-  induction s generalizing r with
-  | nil => rfl
-  | cons x xs ih =>
-    simp [injs']
-    rw [inj'_flat, ih]
-
-theorem injs_flat {r : Regex α} {s : List α} {v : Value α} (hv : Inhab v (r.derivs s)) :
-  (injs r s ⟨v, hv⟩).fst.flat = s ++ v.flat := by
+theorem injs_flat {r : Regex α} {s : List α} {p : Parse (r.derivs s)} :
+  (injs s p).flat = s ++ p.flat := by
   induction s generalizing r with
   | nil => rfl
   | cons x xs ih =>
     simp [injs]
-    rw [inj_flat, ih hv]
+    rw [inj_flat, ih]
 
-def Regex.parse' : (r : Regex α) → List α → Option (Parse r)
+def Regex.parse : (r : Regex α) → List α → Option (Parse r)
   | r, s =>
     let r' := r.derivs s
     if h : r'.nullable
-      then some (injs' s (mkeps' h))
+      then some (injs s (mkeps h))
       else none
 
-def Regex.parse : Regex α → List α → Option (Value α)
-  | r, s =>
-    let r' := r.derivs s
-    if h : r'.nullable
-      then some (injs r s (r'.mkeps h)).fst
-      else none
-
-theorem parse_flat {r : Regex α} {s : List α} {v : Value α} :
-  r.parse s = some v → v.flat = s := by
+theorem parse_flat {r : Regex α} {s : List α} {p : Parse r} :
+  r.parse s = some p → p.flat = s := by
   intro h
   simp [parse] at h
   rcases h with ⟨hn, h⟩
   rw [←h, injs_flat, mkeps_flat]
   exact List.append_nil s
-
-theorem parse'_flat {r : Regex α} {s : List α} {p : Parse r} :
-  r.parse' s = some p → p.flat = s := by
-  intro h
-  simp [parse'] at h
-  rcases h with ⟨hn, h⟩
-  rw [←h, injs'_flat, mkeps'_flat]
-  exact List.append_nil s
-
-theorem parse_matches_iff {r : Regex α} (s : List α) :
-  (r.parse s).isSome ↔ r.Matches s := by
-  induction s generalizing r with
-  | nil =>
-    rw [←nullable_iff_matches_nil]
-    simp [parse]
-  | cons x xs ih =>
-    rw [Matches.deriv_iff, ←ih]
-    simp [parse]
