RegexPosix/Value.lean
@@ -4,28 +4,8 @@ import Mathlib.Data.Bool.Basic
 
 universe u
 
-inductive Value (α : Type u)
-  | empty : Value α
-  | char : α → Value α
-  | left : Value α → Value α
-  | right : Value α → Value α
-  | seq : Value α → Value α → Value α
-  | stars : List (Value α) → Value α
-  deriving Repr
-
 variable {α : Type u}
 
-@[simp]
-def Value.flat : Value α → List α
-  | empty => []
-  | char c => [c]
-  | left v => v.flat
-  | right v => v.flat
-  | seq v₁ v₂ => v₁.flat ++ v₂.flat
-  | stars [] => []
-  | stars (v::vs) => v.flat ++ (stars vs).flat
-
-open Value
 open Regex
 
 inductive Parse : Regex α → Type u
@@ -47,6 +27,11 @@ inductive Parse : Regex α → Type u
     Parse r →
     Parse r.star →
     Parse r.star
+
+def Parse.cast {r₁ r₂ : Regex α} (h : r₁ = r₂) (p : Parse r₁) : Parse r₂ :=
+  h ▸ p
+
+def Parse.cast_rfl {r : Regex α} {p : Parse r} : p.cast rfl = p := rfl
 
 protected def Parse.repr [Repr α] {r : Regex α} (p : Parse r) (n : Nat) : Std.Format :=
   let _ : Std.ToFormat α := ⟨repr⟩
@@ -84,36 +69,6 @@ def Parse.flat {r : Regex α} : Parse r → List α
   | star_nil => []
   | star_cons p ps => p.flat ++ ps.flat
 
-inductive Inhab : Value α → Regex α → Prop
-  | empty : Inhab empty epsilon
-  | char (c : α) : Inhab (char c) (char c)
-  | left {v₁ : Value α} {r₁ r₂ : Regex α} :
-    Inhab v₁ r₁ →
-    Inhab (left v₁) (plus r₁ r₂)
-  | right {v₂ : Value α} {r₁ r₂ : Regex α} :
-    Inhab v₂ r₂ →
-    Inhab (right v₂) (plus r₁ r₂)
-  | seq {v₁ v₂ : Value α} {r₁ r₂ : Regex α} :
-    Inhab v₁ r₁ →
-    Inhab v₂ r₂ →
-    Inhab (seq v₁ v₂) (mul r₁ r₂)
-  | star_nil {r : Regex α} :
-    Inhab (stars []) (star r)
-  | stars {v : Value α} {vs : List (Value α)} {r : Regex α} :
-    Inhab v r →
-    Inhab (stars vs) (star r) →
-    Inhab (stars (v::vs)) (star r)
-
-theorem Inhab.matches {r : Regex α} {v : Value α} :
-  Inhab v r → r.Matches v.flat
-  | empty => (Value.flat.eq_def _) ▸ Matches.epsilon
-  | char c => (Value.flat.eq_def _) ▸ Matches.char
-  | left h => (Value.flat.eq_def _) ▸ h.matches.left
-  | right h => (Value.flat.eq_def _) ▸ h.matches.right
-  | seq h₁ h₂ => (Value.flat.eq_def _) ▸ Matches.mul rfl h₁.matches h₂.matches
-  | star_nil => (Value.flat.eq_def _) ▸ Matches.star_nil
-  | stars h₁ h₂ => (Value.flat.eq_def _) ▸ Matches.stars rfl h₁.matches h₂.matches
-
 theorem Parse.matches {r : Regex α} :
   (p : Parse r) → r.Matches p.flat
   | empty => Matches.epsilon
@@ -124,115 +79,26 @@ theorem Parse.matches {r : Regex α} :
   | star_nil => Matches.star_nil
   | star_cons p ps => Matches.stars rfl p.matches ps.matches
 
-theorem matches_inhab {r : Regex α} {s : List α} :
-  r.Matches s → ∃ v, v.flat = s ∧ Inhab v r := by
+theorem matches_parse {r : Regex α} {s : List α} :
+  r.Matches s → ∃ p : Parse r, p.flat = s := by
   intro h
   induction h with
-  | epsilon => exact ⟨Value.empty, by simp, Inhab.empty⟩
-  | char => exact ⟨Value.char _, by simp, Inhab.char _⟩
+  | epsilon => exact ⟨Parse.empty, rfl⟩
+  | char => exact ⟨Parse.char _, rfl⟩
   | left h ih =>
-    rcases ih with ⟨v, hv, ih⟩
-    exact ⟨v.left, by simp [hv], ih.left⟩
+    rcases ih with ⟨p, hp⟩
+    exact ⟨p.left, hp⟩
   | right h ih =>
-    rcases ih with ⟨v, hv, ih⟩
-    exact ⟨v.right, by simp [hv], ih.right⟩
+    rcases ih with ⟨p, hp⟩
+    exact ⟨p.right, hp⟩
   | mul hs h₁ h₂ ih₁ ih₂ =>
-    rcases ih₁ with ⟨v₁, hv₁, ih₁⟩
-    rcases ih₂ with ⟨v₂, hv₂, ih₂⟩
-    exact ⟨v₁.seq v₂, by simp [hv₁, hv₂, hs], ih₁.seq ih₂⟩
-  | star_nil => exact ⟨Value.stars [], by simp, Inhab.star_nil⟩
+    subst hs
+    rcases ih₁ with ⟨p₁, hp₁⟩
+    rcases ih₂ with ⟨p₂, hp₂⟩
+    exact ⟨p₁.seq p₂, congr_arg₂ (·++·) hp₁ hp₂⟩
+  | star_nil => exact ⟨Parse.star_nil, rfl⟩
   | stars hs h₁ h₂ ih₁ ih₂ =>
-    rcases ih₁ with ⟨v, hv, ih₁⟩
-    rcases ih₂ with ⟨vs, hvs, ih₂⟩
-    match vs with
-    | Value.stars vs =>
-      exact ⟨Value.stars (v::vs), by simp [hv, hvs, hs], Inhab.stars ih₁ ih₂⟩
-
-@[simp]
-theorem inhab_zero {v : Value α} :
-  ¬Inhab v emptyset := by
-  intro h
-  cases h
-
-theorem inhab_left {v₁ : Value α} {r₁ r₂ : Regex α} :
-  Inhab (left v₁) (plus r₁ r₂) → Inhab v₁ r₁ := by
-  intro h
-  cases h with
-  | left h =>
-    exact h
-
-theorem inhab_right {v₂ : Value α} {r₁ r₂ : Regex α} :
-  Inhab (right v₂) (plus r₁ r₂) → Inhab v₂ r₂ := by
-  intro h
-  cases h with
-  | right h =>
-    exact h
-
-theorem inhab_seq {v₁ v₂ : Value α} {r₁ r₂ : Regex α} :
-  Inhab (seq v₁ v₂) (mul r₁ r₂) → Inhab v₁ r₁ ∧ Inhab v₂ r₂ := by
-  intro h
-  cases h with
-  | seq h₁ h₂ => exact ⟨h₁, h₂⟩
-
-theorem inhab_seq_fst {v₁ v₂ : Value α} {r₁ r₂ : Regex α} :
-  Inhab (seq v₁ v₂) (mul r₁ r₂) → Inhab v₁ r₁ := by
-  intro h
-  cases h with
-  | seq h₁ _ => exact h₁
-
-theorem inhab_seq_snd {v₁ v₂ : Value α} {r₁ r₂ : Regex α} :
-  Inhab (seq v₁ v₂) (mul r₁ r₂) → Inhab v₂ r₂ := by
-  intro h
-  cases h with
-  | seq _ h₂ => exact h₂
-
-theorem inhab_stars_head {v : Value α} {vs : List (Value α)} {r : Regex α} :
-  Inhab (stars (v::vs)) (star r) → Inhab v r := by
-  intro h
-  cases h with
-  | stars h₁ _ => exact h₁
-
-theorem inhab_stars_tail {v : Value α} {vs : List (Value α)} {r : Regex α} :
-  Inhab (stars (v::vs)) (star r) → Inhab (stars vs) r.star := by
-  intro h
-  cases h with
-  | stars _ h₂ => exact h₂
-
-theorem  Inhab_not_nullable {r : Regex α} {v : Value α} (hn : ¬r.nullable) (hv : v.flat = []) :
-  ¬Inhab v r := by
-  intro h
-  induction r generalizing v with
-  | emptyset => nomatch h
-  | epsilon => simp at hn
-  | char =>
-    cases h with
-    | char => simp at hv
-  | plus r₁ r₂ ih₁ ih₂ =>
-    simp at hn
-    cases h with
-    | left h =>
-      apply ih₁
-      simp [hn]
-      simp at hv
-      exact hv
-      exact h
-    | right h =>
-      apply ih₂
-      simp [hn]
-      simp at hv
-      exact hv
-      exact h
-  | mul r₁ r₂ ih₁ ih₂ =>
-    cases h with
-    | seq h₁ h₂ =>
-      simp at hv
-      simp at hn
-      apply ih₁
-      intro hn₁
-      apply ih₂
-      simp [hn hn₁]
-      exact hv.right
-      exact h₂
-      exact hv.left
-      exact h₁
-  | star r => simp at hn
+    subst hs
+    rcases ih₁ with ⟨p, hp⟩
+    rcases ih₂ with ⟨ps, hps⟩
+    exact ⟨p.star_cons ps, congr_arg₂ (·++·) hp hps⟩
