RegexPosix/Correctness.lean
@@ -2,70 +2,43 @@ import RegexPosix.POSIX
 import RegexPosix.Parse
 
 open Regex
-open Value
+open Parse
 
 universe u
 
 variable {α : Type u}
 
-theorem mkeps'_posix {r : Regex α} {hn : r.nullable} :
-  POSIX' (mkeps' hn) := by
-  fun_induction mkeps' with
-  | case1 => exact POSIX'.epsilon
+theorem mkeps_posix {r : Regex α} {hn : r.nullable} :
+  POSIX (mkeps hn) := by
+  fun_induction mkeps with
+  | case1 => exact POSIX.epsilon
   | case2 r₁ r₂ hn hn₁ ih₁ =>
-    exact POSIX'.left ih₁
+    exact POSIX.left ih₁
   | case3 r₁ r₂ hn hn₁ hn₂ ih₂ =>
-    refine POSIX'.right ih₂ ?_
-    rw [mkeps'_flat]
+    refine POSIX.right ih₂ ?_
+    rw [mkeps_flat]
     rw [←nullable_iff_matches_nil]
     exact hn₁
   | case4 r₁ r₂ hn hn₁ hn₂ ih₁ ih₂ =>
-    exact POSIX'.mul ih₁ ih₂ (by simp [mkeps'_flat])
-  | case5 r hn => exact POSIX'.star_nil
-
-theorem mkeps_posix {r : Regex α} (hn : r.nullable) :
-  POSIX r (r.mkeps hn).fst := by
-  induction r with
-  | emptyset => simp [nullable] at hn
-  | epsilon =>
-    simp only [mkeps]
-    apply POSIX.epsilon
-  | char => simp [nullable] at hn
-  | plus r₁ r₂ ih₁ ih₂ =>
-    simp at hn
-    simp only [mkeps]
-    split_ifs with hn'
-    · exact POSIX.left (ih₁ hn')
-    · refine POSIX.right (ih₂ (Or.resolve_left hn hn')) ?_
-      rw [mkeps_flat]
-      rw [←nullable_iff_matches_nil]
-      exact hn'
-  | mul r₁ r₂ ih₁ ih₂ =>
-    simp at hn
-    simp only [mkeps]
-    refine POSIX.mul (ih₁ hn.left) (ih₂ hn.right) ?_
-    rw [mkeps_flat]
-    simp_all
-  | star r ih =>
-    simp only [mkeps]
-    apply POSIX.star_nil
+    exact POSIX.mul ih₁ ih₂ (by simp [mkeps_flat])
+  | case5 r hn => exact POSIX.star_nil
 
 variable [DecidableEq α]
 
-theorem inj'_posix {r : Regex α} {c : α} {p : Parse (r.deriv c)} (h : POSIX' p) :
-  POSIX' (inj' c p) := by
-  fun_induction inj' with
+theorem inj_posix {r : Regex α} {c : α} {p : Parse (r.deriv c)} (h : POSIX p) :
+  POSIX (inj c p) := by
+  fun_induction inj with
   | case1 d c p =>
-    exact POSIX'.char d
+    exact POSIX.char d
   | case2 r₁ r₂ c p ih₁ =>
     cases h with
     | left h =>
-      exact POSIX'.left (ih₁ h)
+      exact POSIX.left (ih₁ h)
   | case3 r₁ r₂ c p ih₂ =>
     cases h with
     | right h hn =>
-      refine POSIX'.right (ih₂ h) ?_
-      rw [inj'_flat, Matches.deriv_iff]
+      refine POSIX.right (ih₂ h) ?_
+      rw [inj_flat, Matches.deriv_iff]
       exact hn
   | case4 r₁ r₂ c hn₁ p₁ p₂ p heq ih₁ =>
     generalize_proofs k at heq
@@ -76,8 +49,8 @@ theorem inj'_posix {r : Regex α} {c : α} {p : Parse (r.deriv c)} (h : POSIX' p
     | left h =>
       cases h with
       | mul h₁ h₂ hs =>
-        refine POSIX'.mul (ih₁ h₁) h₂ ?_
-        simp_rw [inj'_flat, List.cons_append, Matches.deriv_iff]
+        refine POSIX.mul (ih₁ h₁) h₂ ?_
+        simp_rw [inj_flat, List.cons_append, Matches.deriv_iff]
         exact hs
   | case5 r₁ r₂ c hn₁ p₂ p heq ih₂ =>
     generalize_proofs k at heq
@@ -86,8 +59,8 @@ theorem inj'_posix {r : Regex α} {c : α} {p : Parse (r.deriv c)} (h : POSIX' p
     subst hr heq
     cases h with
     | right h hn =>
-      refine POSIX'.mul (mkeps'_posix) (ih₂ h) ?_
-      simp [inj'_flat, mkeps'_flat]
+      refine POSIX.mul (mkeps_posix) (ih₂ h) ?_
+      simp [inj_flat, mkeps_flat]
       intro x hx y hxy hr₁ hr₂
       rw [List.append_eq_cons_iff] at hxy
       simp [hx] at hxy
@@ -102,155 +75,46 @@ theorem inj'_posix {r : Regex α} {c : α} {p : Parse (r.deriv c)} (h : POSIX' p
     subst hr heq
     cases h with
     | mul h₁ h₂ hs =>
-      refine POSIX'.mul (ih₁ h₁) h₂ ?_
-      simp_rw [inj'_flat, List.cons_append, Matches.deriv_iff]
+      refine POSIX.mul (ih₁ h₁) h₂ ?_
+      simp_rw [inj_flat, List.cons_append, Matches.deriv_iff]
       exact hs
   | case7 r c p ps ih =>
     cases h with
     | mul h₁ h₂ hs =>
-      refine POSIX'.stars (ih h₁) h₂ (by simp [inj'_flat]) ?_
-      simp_rw [inj'_flat, List.cons_append, Matches.deriv_iff]
+      refine POSIX.stars (ih h₁) h₂ (by simp [inj_flat]) ?_
+      simp_rw [inj_flat, List.cons_append, Matches.deriv_iff]
       exact hs
 
-theorem inj_posix {r : Regex α} {v : Value α} {c : α} (h : POSIX (r.deriv c) v) :
-  POSIX r (inj r c ⟨v, h.inhab⟩).fst := by
-  induction r generalizing v with
-  | emptyset =>
-    simp at h
-    cases h
-  | epsilon =>
-    simp at h
-    cases h
-  | char d =>
-    simp [deriv] at h
-    split_ifs at h with hc
-    · cases h
-      simp [hc] at h
-      simp [inj]
-      exact POSIX.char d
-    · cases h
-  | plus r₁ r₂ ih₁ ih₂ =>
-    match v with
-    | Value.left v' =>
-      cases h with
-      | left h =>
-        simp [inj]
-        exact POSIX.left (ih₁ h)
-    | Value.right v' =>
-      cases h with
-      | right h hn =>
-        simp [inj]
-        refine POSIX.right (ih₂ h) ?_
-        rw [inj_flat, Matches.deriv_iff]
-        exact hn
-  | mul r₁ r₂ ih₁ ih₂ =>
-    simp [deriv] at h
-    split_ifs at h with hn
-    · cases h with
-      | left h' =>
-        simp [hn] at h
-        cases h' with
-        | mul h₁ h₂ hs =>
-          simp [inj, hn]
-          refine POSIX.mul (ih₁ h₁) h₂ ?_
-          simp_rw [inj_flat, List.cons_append, Matches.deriv_iff]
-          exact hs
-      | right h' hn' =>
-        simp [inj, hn]
-        refine POSIX.mul (mkeps_posix hn) (ih₂ h') ?_
-        simp
-        intro x hx y hxy hr₁ hr₂
-        rw [inj_flat] at hxy
-        simp [mkeps_flat] at hr₁
-        rw [List.append_eq_cons_iff] at hxy
-        simp [hx] at hxy
-        rcases hxy with ⟨z, hx, hs⟩
-        rw [hx, Matches.deriv_iff] at hr₁
-        rw [hs] at hn'
-        exact absurd (Matches.mul rfl hr₁ hr₂) hn'
-    · cases h with
-      | mul h₁ h₂ hn' =>
-        simp [inj, hn]
-        refine POSIX.mul (ih₁ h₁) h₂ ?_
-        simp_rw [inj_flat, List.cons_append, Matches.deriv_iff]
-        exact hn'
-  | star r ih =>
-    match v with
-    | Value.seq v (Value.stars vs) =>
-      simp [inj]
-      cases h with
-      | mul h₁ h₂ hs =>
-        refine POSIX.stars (ih h₁) h₂ (by simp [inj_flat]) ?_
-        simp_rw [inj_flat, List.cons_append, Matches.deriv_iff]
-        exact hs
-
-theorem injs'_posix {r : Regex α} {s : List α} {p : Parse (r.derivs s)} (h : POSIX' p) :
-  POSIX' (injs' s p) := by
+theorem injs_posix {r : Regex α} {s : List α} {p : Parse (r.derivs s)} (h : POSIX p) :
+  POSIX (injs s p) := by
   induction s generalizing r with
   | nil =>
     exact h
   | cons x xs ih =>
-    rw [injs']
-    exact inj'_posix (ih h)
-
-theorem injs_posix {r : Regex α} {v : Value α} {s : List α} (h : POSIX (r.derivs s) v) :
-  POSIX r (injs r s ⟨v, h.inhab⟩).fst := by
-  induction s generalizing r with
-  | nil =>
-    rw [derivs] at h
-    exact h
-  | cons x xs ih =>
-    rw [derivs] at h
-    simp [injs]
-    apply inj_posix
-    exact ih h
-
-theorem matches_parse'_posix_iff {r : Regex α} {s : List α} :
-  r.Matches s ↔ ∃ p, r.parse' s = some p ∧ POSIX' p := by
-  simp [parse']
-  rw [Matches.derivs_iff, ←nullable_iff_matches_nil]
-  constructor
-  · intro h
-    exact ⟨h, injs'_posix mkeps'_posix⟩
-  · intro ⟨h, _⟩
-    exact h
+    rw [injs]
+    exact inj_posix (ih h)
 
 theorem matches_parse_posix_iff {r : Regex α} {s : List α} :
-  r.Matches s ↔ ∃ v, r.parse s = some v ∧ POSIX r v := by
+  r.Matches s ↔ ∃ p, r.parse s = some p ∧ POSIX p := by
   simp [parse]
   rw [Matches.derivs_iff, ←nullable_iff_matches_nil]
   constructor
   · intro h
-    exact ⟨h, injs_posix (mkeps_posix h)⟩
+    exact ⟨h, injs_posix mkeps_posix⟩
   · intro ⟨h, _⟩
     exact h
 
-theorem parse_posix_iff (r : Regex α) (s : List α) (v : Value α) :
-  r.parse s = some v ↔ v.flat = s ∧ POSIX r v := by
+theorem parse_posix_iff (r : Regex α) (s : List α) (p : Parse r) :
+  r.parse s = some p ↔ p.flat = s ∧ POSIX p := by
   constructor
   · intro h
     refine ⟨parse_flat h, ?_⟩
     simp [parse] at h
     rcases h with ⟨hn, h⟩
     rw [←h]
-    exact injs_posix (mkeps_posix hn)
+    exact injs_posix mkeps_posix
   · intro ⟨hv, h⟩
     subst hv
     rcases (matches_parse_posix_iff.mp h.matches) with ⟨v', h', h''⟩
     rw [POSIX.unique (parse_flat h') h'' h] at h'
-    exact h'
-
-theorem parse'_posix_iff (r : Regex α) (s : List α) (p : Parse r) :
-  r.parse' s = some p ↔ p.flat = s ∧ POSIX' p := by
-  constructor
-  · intro h
-    refine ⟨parse'_flat h, ?_⟩
-    simp [parse'] at h
-    rcases h with ⟨hn, h⟩
-    rw [←h]
-    exact injs'_posix mkeps'_posix
-  · intro ⟨hv, h⟩
-    subst hv
-    rcases (matches_parse'_posix_iff.mp h.matches) with ⟨v', h', h''⟩
-    rw [POSIX'.unique (parse'_flat h') h'' h] at h'
     exact h'
